theories/Playground/UnsafeSim.v
@@ -1,0 +1,77 @@
+From RSL Require Import Prelude.
+
+From RSL.Commons Require Export Language Behaviors.
+
+From Coinduction Require Import all.
+
+Section USimDef.
+  Context {Λt Λs: lang}.
+  Context (Pt: prog Λt) (Ps: prog Λs).
+  Context (Φ: value Λt -> value Λs -> memory -> memory -> Prop).
+
+  Variant usim_lfp' (gfp: state Λt -> state Λs -> Prop)
+    : state Λt -> state Λs -> Prop :=
+  | URelated : ∀ t s,
+    both_final Φ t s -> usim_lfp' gfp t s
+
+  | UTargetSteps : ∀ t s,
+    can_progress Pt t ->
+    (∀ t', Pt ⊨ t ->> t' -> gfp t' s) ->
+    usim_lfp' gfp t s
+
+  | USourceSteps : ∀ t s s',
+    Ps ⊨ s ->> s' ->
+    gfp t s' ->
+    usim_lfp' gfp t s.
+
+  Program Definition usim_lfp : mon (state Λt -> state Λs -> Prop) :=
+    {| body := usim_lfp' |}.
+  Next Obligation.
+    intros gfp gfp' Hgfp t s Hsim.
+    induction Hsim as [ | ? ? Hprog Ht | ? ? ? Hstep Hs ].
+    - now constructor.
+    - eapply UTargetSteps; eauto.
+      intros t' Hstep.
+      by apply Hgfp, Ht.
+    - eapply USourceSteps; eauto.
+      by apply Hgfp, Hs.
+  Qed.
+
+  Lemma usim_unroll t s :
+    gfp usim_lfp t s -> usim_lfp' (gfp usim_lfp) t s.
+  Proof using Type. apply (gfp_fp usim_lfp). Qed.
+
+  Lemma usim_roll t s :
+    usim_lfp' (gfp usim_lfp) t s -> gfp usim_lfp t s.
+  Proof using Type. apply (gfp_fp usim_lfp). Qed.
+
+  Definition usim := gfp usim_lfp.
+
+  Lemma loop_target t :
+    strong_diverge Pt t ->
+    ∀ s, usim t s.
+  Proof using Type.
+    unfold usim.
+    revert t.
+    coinduction C CIH.
+    intros t Hdiv s.
+    apply UTargetSteps.
+    - by apply Hdiv.
+    - intros u Hstep.
+      apply CIH.
+      intros t' Hrtc.
+      apply Hdiv. by econstructor.
+  Qed.
+
+  Lemma loop_source s :
+    diverges Ps s ->
+    ∀ t, usim t s.
+  Proof using Type.
+    unfold usim.
+    revert s.
+    coinduction C CIH.
+    intros s (s' & Hstep & Hdiv)%diverges_unroll t.
+    eapply USourceSteps; first done.
+    by apply CIH.
+  Qed.
+End USimDef.
