theories/Simulations/LockStep.v
@@ -1,0 +1,44 @@
+From RSL Require Import Prelude.
+
+From RSL.Commons Require Export Language.
+
+From Coinduction Require Import all.
+
+Section LSimDef.
+  Context {Λt Λs: lang}.
+  Context (Pt: prog Λt) (Ps: prog Λs).
+  Context (Φ: value Λt -> value Λs -> memory -> memory -> Prop).
+
+  Variant lsim_lfp' (gfp: state Λt -> state Λs -> Prop)
+    : state Λt -> state Λs -> Prop :=
+  | LRelated : ∀ t s,
+    both_final Φ t s -> lsim_lfp' gfp t s
+
+  | LBothSteps : ∀ t s,
+    can_progress Pt t ->
+    (∀ t', Pt ⊨ t ->> t' -> ∃ s', Ps ⊨ s ->> s' ∧ gfp t' s') ->
+    lsim_lfp' gfp t s.
+
+  Program Definition lsim_lfp : mon (state Λt -> state Λs -> Prop) :=
+    {| body := lsim_lfp' |}.
+  Next Obligation.
+    intros gfp gfp' Hgfp t s Hsim.
+    induction Hsim as [ | ? ? Hprog Hboth].
+    - now constructor.
+    - eapply LBothSteps; eauto.
+      intros t' Hstep.
+      destruct (Hboth _ Hstep) as (s' & ? & ?).
+      exists s'. split; auto.
+      now apply Hgfp.
+  Qed.
+
+  Lemma lsim_unroll t s :
+    gfp lsim_lfp t s -> lsim_lfp' (gfp lsim_lfp) t s.
+  Proof using Type. apply (gfp_fp lsim_lfp). Qed.
+
+  Lemma lsim_roll t s :
+    lsim_lfp' (gfp lsim_lfp) t s -> gfp lsim_lfp t s.
+  Proof using Type. apply (gfp_fp lsim_lfp). Qed.
+
+  Definition lsim  := gfp lsim_lfp.
+End LSimDef.
