theories/Simulations/Soundness/LockSound.v
@@ -1,0 +1,147 @@
+From RSL Require Import Prelude.
+
+From Stdlib Require Import Classical.
+From Coinduction Require Import all.
+
+From RSL Require Import Commons.Behaviors.
+From RSL Require Import Simulations.LockStep.
+
+Section LSimSound.
+  Context {Λt Λs: lang}.
+  Context (Pt: prog Λt) (Ps: prog Λs).
+
+  Instance beht_elem : ElemOf behavior (state Λt) := beh Pt.
+  Instance behs_elem : ElemOf behavior (state Λs) := beh Ps.
+
+  Notation "a '≡{' Φ '}' b" :=
+    (behavior_equal Φ a b)
+      (at level 70, format "a  '≡{' Φ '}'  b", no associativity).
+
+  Notation "t '≲' s '{{' Φ '}}'" :=
+    (lsim Pt Ps Φ t s)
+      (at level 1, no associativity).
+
+  Lemma terminating_lsim Φ t s:
+    t ≲ s {{ Φ }} ->
+    ∀ vt mt,
+    Terminating vt mt ∈ t ->
+    ∃ b, b ∈ s ∧ Terminating vt mt ≡{Φ} b.
+  Proof using Type.
+    intros Hsim vt mt Hb.
+    (* t Terminates -> it reduces to a final state *)
+    apply has_terminating_behavior in Hb. destruct Hb as (t' & Hrtc & Hfin).
+    revert s Hsim.
+    (* Induction on the reduction *)
+    induction Hrtc as [ t | t u t' Ht Hrtc IHt ].
+    - (* t is final *)
+      intros s Hsim.
+      (* Induction on the least-fixpoint of the relation *)
+      apply lsim_unroll in Hsim.
+      induction Hsim as [ t s Hfinal
+                        | t s Hprogress Hboth ].
+      + (* Both Final *)
+        destruct Hfinal as (? & vs & ? & ms & Ht & ? & ?).
+        (* s is final too *)
+        inv Ht. exists (Terminating vs ms). by do 2 constructor.
+      + (* Both Steps -> contradiction *)
+        langmixin.
+    - (* t steps *)
+      intros s Hsim.
+      (* Induction on the least-fixpoint of the relation *)
+      apply lsim_unroll in Hsim.
+      induction Hsim as [ t s Hfinal
+                        | t s Hprogress IHboth ].
+      + (* Both Final -> contradiction *)
+        langmixin.
+      + (* Both Steps, use IH on t *)
+        destruct (IHboth _ Ht) as (s' & Hs & Hgfp).
+        edestruct IHt as (b & Hbeh & ?); eauto.
+        exists b. split; auto.
+        eapply IsSteping; now eauto.
+  Qed.
+
+  Lemma lsim_lfp_progress Φ t s:
+    t ≲ s {{ Φ }} ->
+    diverges Pt t ->
+    ∃ t' s', Ps ⊨ s ->> s' ∧ t' ≲ s' {{ Φ }} ∧ diverges Pt t'.
+  Proof using Type.
+    intros Hsim Hdiv.
+    (* Induction on the least-fixpoint of the relation *)
+    apply lsim_unroll in Hsim.
+    induction Hsim as [ t s Hfinal
+                      | t s Hprogress IHboth ].
+    - (* Both Final: Contradiction *)
+      apply diverges_unroll in Hdiv. destruct Hdiv as (t' & Ht_step & _).
+      langmixin.
+    - (* Both Steps *)
+      apply diverges_unroll in Hdiv. destruct Hdiv as (t' & Ht_step & Hdiv_t').
+      (* Use IH on t to make s steps *)
+      destruct (IHboth t' Ht_step) as (s' & Hstep & Hgfp).
+      exists t', s'. now auto.
+  Qed.
+
+  Lemma diverging_lsim Φ t s:
+    t ≲ s {{ Φ }} ->
+    Diverging ∈ t ->
+    Diverging ∈ s.
+  Proof using Type.
+    intros Hsim Hdiv. constructor.
+    apply has_diverging_behavior in Hdiv.
+    (* We prove by coinduction that s diverges *)
+    unfold diverges.
+    revert t s Hdiv Hsim. coinduction ξ cih.
+    intros t s Hdiv Hsim.
+    (* [sim_lfp_progress] give us s' such that s ->> s' *)
+    destruct (lsim_lfp_progress _ _ _ Hsim Hdiv) as (t' & s' & Hstep & Hsim' & Hdiv').
+    (* s steps *)
+    exists s'. split; auto. eapply cih; now eauto.
+  Qed.
+
+  Lemma undef_lsim Φ t s:
+    t ≲ s {{ Φ }} ->
+    Undef ∈ t ->
+    Undef ∈ s.
+  Proof using Type.
+    intros Hsim Hb.
+    (* t reach a stuck state. *)
+    apply has_undef_behavior in Hb. destruct Hb as (t' & Hrtc & Hstuck).
+    revert s Hsim.
+    (* Induction on the reduction *)
+    induction Hrtc as [ t | t u t' Htstep Hrtc IHt ].
+    - (* t = t' *)
+      intros s Hsim.
+      (* Induction on the least-fixpoint of the relation *)
+      apply lsim_unroll in Hsim.
+      induction Hsim as [ t s Hfinal
+                        | t s Hprogress _ ].
+      + (* Both Final -> contradiction *)
+        langmixin.
+      + (* Both Steps -> contradiction *)
+        langmixin.
+    - (* t steps *)
+      intros s Hsim.
+      (* Induction on the least-fixpoint of the relation *)
+      apply lsim_unroll in Hsim.
+      induction Hsim as [ t s Hfinal
+                        | t s Hprogress Hboth ].
+      + (* Both Final -> contradiction *)
+        langmixin.
+      + (* Both Steps, use IH on t *)
+        destruct (Hboth _ Htstep) as (s' & Hstep & Hgfp).
+        apply IHt in Hgfp; auto.
+        eapply IsSteping; now eauto.
+  Qed.
+
+  Theorem lsim_sound Φ t s:
+    t ≲ s {{ Φ }} -> rigid_refines Pt Ps Φ t s.
+  Proof using Type.
+    intros Hsim [] Hb.
+    - eapply terminating_lsim; now eauto.
+    - exists Diverging. split.
+      + eapply diverging_lsim; now eauto.
+      + now constructor.
+    - exists Undef. split.
+      + eapply undef_lsim; now eauto.
+      + now constructor.
+  Qed.
+End LSimSound.
